\documentclass[16pt]{article}

\usepackage{array,amsmath,amssymb,amsthm,amsfonts,amscd}
\usepackage{showlabels}
\usepackage{color}
\usepackage{hyperref}
\usepackage[numeric]{amsrefs}
\usepackage{graphicx}

\usepackage[framemethod=TikZ]{mdframed}
%\usepackage[framemethod=default]{mdframed}


%\mdfdefinestyle{box}{%
%rightline=true,
%innerleftmargin=10,
%innerrightmargin=10,
%frametitlerule=true,
%frametitlerulecolor=blue,
%frametitlebackgroundcolor=white,
%frametitlerulewidth=2pt}

\mdfdefinestyle{TheoremFrame}{%
    linecolor=blue,
    outerlinewidth=1,
    roundcorner=15,
    innertopmargin= \baselineskip,
    innerbottommargin= \baselineskip,
    innerrightmargin=10,
    innerleftmargin=10,
    backgroundcolor=white}
    
\mdfdefinestyle{ProofFrame}{%
    linecolor=red,
    outerlinewidth=1,
    roundcorner=15,
    innertopmargin= \baselineskip,
    innerbottommargin= \baselineskip,
    innerrightmargin=10,
    innerleftmargin=10,
    backgroundcolor=white}
    
    
\setlength{\oddsidemargin}{0cm}
\setlength{\evensidemargin}{0cm}
\setlength{\marginparwidth}{0in}
\setlength{\marginparsep}{0in}
\setlength{\marginparpush}{0in}
\setlength{\topmargin}{0in}
\setlength{\headheight}{0pt}
\setlength{\headsep}{0pt}
\setlength{\footskip}{.3in}
\setlength{\textheight}{9.2in}
\setlength{\textwidth}{6.0in}
\setlength{\parskip}{0.25pt}
\setlength{\parindent}{0.25in}

    
\newlength\tindent
\setlength{\tindent}{\parindent}
\setlength{\parindent}{0pt}
\renewcommand{\indent}{\hspace*{\tindent}}

\newtheorem*{nthm}{Theorem}
\newtheorem*{nlem}{Lemma}
\newtheorem*{nprop}{Proposition}
\newtheorem*{ncor}{Corollary}
\newtheorem*{nconj}{Conjecture}
\newtheorem*{nclaim}{Claim}
\theoremstyle{remark}
\newtheorem*{define}{Definition}
\newtheorem*{nrem}{Remarks}
\newtheorem*{notation}{Notation}
\newtheorem*{note}{Note}
\newtheorem*{ex}{Example}
\newtheorem*{imt}{Important}
\newtheorem*{fact}{Fact}
\newcommand{\vs}{\vspace{0.1in}}
\newcommand{\Lim}[1]{\raisebox{0.5ex}{\scalebox{0.8}{$\displaystyle \lim_{#1}\;$}}}
\newcolumntype{M}[1]{>{\centering\arraybackslash}m{#1}}
\newcolumntype{N}{@{}m{0pt}@{}}
\renewcommand{\arraystretch}{2.5}
\title{Exponents}

\author{Stephen Styles}


\begin{document}
\maketitle

Laws of Exponents:\\

\begin{table}[h!]
\centering
\caption{For $a\not= 0$, $b \not= 0$}
\begin{tabular}{||>{\centering\arraybackslash}m{1.5in} | M{1.5in}|| N } 
 \hline
 Product Rule & $\displaystyle{a^x \cdot a^y = a^{x+y}}$ &\\
 \hline
 Quotient Rule & $\displaystyle{\frac{a^x}{a^y}=a^{x-y}}$&\\
 \hline
 Power Rule & $\displaystyle{(a^x)^y = a^{xy}}$\\
 \hline
 Power of a Product Rule & $\displaystyle{(ab)^x = a^x b^x}$&\\ 
 \hline
 Power of a Fraction Rule & $\displaystyle{\bigg(\frac{a}{b}\bigg)^x = \frac{a^x}{b^x}}$&\\
 \hline
 Zero Exponent &$\displaystyle{a^0 = 1}$&\\
 \hline
 Negative Exponent & $\displaystyle{a^{-x} = \frac{1}{a^x}}$ &\\
 \hline
 Fractional Exponent & $\displaystyle{a^{x/y} = \sqrt[y]{a^x}}$&\\
 \hline
\end{tabular}
\end{table}

Examples:
\begin{enumerate}
\item  Write $\displaystyle{\frac{3^3 \cdot 3^2 \cdot 3^{-1}}{3^6}}$ in the simplest form.
\begin{mdframed}[style=TheoremFrame]
\textit{Solution}:
\begin{align*}
\frac{3^3 \cdot 3^2 \cdot 3^{-1}}{3^6} &= 3^{3+2-1-6}\\
&= 3^{-2}\\
&= \frac{1}{3^2}\\
&= \frac{1}{9}
\end{align*}
\end{mdframed}
\newpage
\item Simplify $\displaystyle{2x^3 y^6 \times 8x^5 y^2}$
\begin{mdframed}[style=TheoremFrame]
\textit{Solution:}
\begin{align*}
2x^3 y^6 \times 8x^5 y^2 &= 16x^{3+5} y^{6+2}\\
&= 16 x^8 y^8
\end{align*}
\end{mdframed}
\item Write $\displaystyle{\frac{5^{2/3} \cdot 5^{1/4}}{5^{11/12}}}$ in the simplest form.
\begin{mdframed}[style=TheoremFrame]
\textit{Solution}:
\begin{align*}
\frac{5^{2/3} \cdot 5^{1/4}}{5^{11/12}} &= 5^{2/3 + 1/4 - 11/12}\\
&= 5^{8/12 + 3/12 - 11/12}\\
&= 5^0\\
&=1
\end{align*}
\end{mdframed}
\item Simplify $\displaystyle{\frac{15x^2y^3z^7}{5xy^{-1}z^4}}$
\begin{mdframed}[style=TheoremFrame]
\textit{Solution:}
\begin{align*}
\frac{15x^2y^3z^7}{5xy^{-1}z^4} &= \frac{15}{5} x^{2-1} y^{3 - (-1)} z^{7-4}\\
&= 3 x y^4 z^3
\end{align*}
\end{mdframed}
\end{enumerate}

Questions:
\begin{enumerate}
\item Simplify $3^5 \times 3^2 \times 3^{-4}$
\vspace{5cm}
\newpage
\item Simplify $2^2 \times 2^{-1} \times 2^{-7}$
\vspace{5cm}
\item Simplify $6^7 \times 6^{12} \times 6^{-5} \times 6^9 $
\vspace{5cm}
\item Simplify $7^3 \times 7 \times 7^{-12} \times 7^{14}$
\vspace{5cm}
\item Simplify $2^{10} \times 2^{-9}\times 2^{-6}\times 2^{-2}$
\newpage

\item Simplify $13^4 \times 13^{15} \times 13^{-2} \times 13^6 \times 13^{-9}$
\vspace{5cm}
\item Simplify $x^3 \times x^{4} \times x^{12}  $
\vspace{5cm}
\item Simplify $x^{-3} \times x^5 \times x^{-4} \times x^{-6}$
\vspace{5cm}
\item Simplify $x^{14} \times x^{-21}\times x^{-61}\times x^{34}$
\newpage

\item Simplify $2^5 \times 3^{-5} \times 3^{-4} \times 2^2 \times 3^{7}$
\vspace{5cm}
\item Simplify $4^3 \times 4^{3} \times 5^{6} \times 4^{-7} \times 5^{-3}  $
\vspace{5cm}
\item Simplify $6^{7} \times 7^6 \times 6^{12} \times 7^{-18} \times 6^{-15}$
\vspace{5cm}
\item Simplify $2^{8} \times 3^{-12}\times 2^{9}\times 5^{4} \times 3^{7}$
\newpage


\item Simplify $\displaystyle{\frac{2^5 \times 2^7}{2^4}}$
\vspace{5cm}
\item Simplify $\displaystyle{\frac{x^{-4} \times x^{10}}{x^5 \times x^6}}$
\vspace{5cm}
\item Simplify $\displaystyle{\frac{5^3 \times 5^5 \times 5^2}{5^6 \times 5^9}}$
\vspace{5cm}
\item Simplify $\displaystyle{\frac{2^5 \times 2^7}{2^4}}$
\vspace{5cm}
\newpage

\item Simplify $\displaystyle{\frac{3^3 \times 2^6}{2^3\times 3^5}}$
\vspace{5cm}
\item Simplify $\displaystyle{\frac{x^{6} \times y^{14}}{x^8 \times y^9}}$
\vspace{5cm}
\item Simplify $\displaystyle{\frac{7^3 \times 7^{-2} \times 7^8 \times 7^5}{7^9 \times 7^6}}$
\vspace{5cm}
\item Simplify $\displaystyle{\frac{2^{13}}{2^5\times 2^4 \times 2^8 \times 2^3}}$
\vspace{5cm}
\newpage



\item Write $\displaystyle{\frac{2^3 (4\times 5)^3}{2^5 \times5^4}}$ in the simplest form.
\vspace{5cm}
\item Simplify $\displaystyle{5a^2b^3-\frac{6b^4}{2a^{-2}b}}$
\vspace{5cm}
\item Simplify $\displaystyle{\bigg(\frac{2^2 \times 2^3}{2^2}\bigg)^{1/3} - 3^2\times 3^{-2}}$
\vspace{5cm}

\item Simplify $\displaystyle{\frac{8a^3b^{-2}}{(2a^{-3}b^2)(ab)}}$
\vspace{5cm}
\item Simplify $\displaystyle{(3x^{-3}y^2)(2x^2)(4y^4)^{-2}}$
\vspace{5cm}

\end{enumerate}
\end{document}