\documentclass[16pt]{article}

\usepackage{amsmath,amssymb,amsthm,amsfonts,amscd}
\usepackage{showlabels}
\usepackage{color}
\usepackage{hyperref}
\usepackage[numeric]{amsrefs}
\usepackage{graphicx}

\usepackage[framemethod=TikZ]{mdframed}
%\usepackage[framemethod=default]{mdframed}


%\mdfdefinestyle{box}{%
%rightline=true,
%innerleftmargin=10,
%innerrightmargin=10,
%frametitlerule=true,
%frametitlerulecolor=blue,
%frametitlebackgroundcolor=white,
%frametitlerulewidth=2pt}

\mdfdefinestyle{TheoremFrame}{%
    linecolor=blue,
    outerlinewidth=1,
    roundcorner=15,
    innertopmargin= \baselineskip,
    innerbottommargin= \baselineskip,
    innerrightmargin=10,
    innerleftmargin=10,
    backgroundcolor=white}
    
\mdfdefinestyle{ProofFrame}{%
    linecolor=red,
    outerlinewidth=1,
    roundcorner=15,
    innertopmargin= \baselineskip,
    innerbottommargin= \baselineskip,
    innerrightmargin=10,
    innerleftmargin=10,
    backgroundcolor=white}
    
    
\setlength{\oddsidemargin}{0cm}
\setlength{\evensidemargin}{0cm}
\setlength{\marginparwidth}{0in}
\setlength{\marginparsep}{0in}
\setlength{\marginparpush}{0in}
\setlength{\topmargin}{0in}
\setlength{\headheight}{0pt}
\setlength{\headsep}{0pt}
\setlength{\footskip}{.3in}
\setlength{\textheight}{9.2in}
\setlength{\textwidth}{6.0in}
\setlength{\parskip}{0.25pt}
\setlength{\parindent}{0.25in}

    
\newlength\tindent
\setlength{\tindent}{\parindent}
\setlength{\parindent}{0pt}
\renewcommand{\indent}{\hspace*{\tindent}}

\newtheorem*{nthm}{Theorem}
\newtheorem*{nlem}{Lemma}
\newtheorem*{nprop}{Proposition}
\newtheorem*{ncor}{Corollary}
\newtheorem*{nconj}{Conjecture}
\newtheorem*{nclaim}{Claim}
\theoremstyle{remark}
\newtheorem*{define}{Definition}
\newtheorem*{nrem}{Remarks}
\newtheorem*{notation}{Notation}
\newtheorem*{note}{Note}
\newtheorem*{ex}{Example}
\newtheorem*{imt}{Important}
\newtheorem*{fact}{Fact}
\newcommand{\vs}{\vspace{0.1in}}
\newcommand{\Lim}[1]{\raisebox{0.5ex}{\scalebox{0.8}{$\displaystyle \lim_{#1}\;$}}}


\title{BEDMAS}

\author{Stephen Styles}
\allowdisplaybreaks

\begin{document}

\maketitle
\vspace*{-0.1cm}
BEDMAS is an acronym that reminds us of the correct order of operations:\\
\begin{center}
\begin{tabular}{ l l }
 \textcolor{red}{B}rackets & \textcolor{red}{First Priority}  \\ 
 \textcolor{green}{E}xponents & \textcolor{green}{Second Priority } \\  
 \textcolor{blue}{D}ivision & \textcolor{blue}{Third Priority}  \\
 \textcolor{blue}{M}ultiplication & \textcolor{blue}{Third Priority}\\
 \textcolor{purple}{A}ddition & \textcolor{purple}{Fourth Priority}\\
 \textcolor{purple}{S}ubtraction & \textcolor{purple}{Fourth Priority}\\    
\end{tabular}
\end{center}
This acronym tells us which order to evaluate our expressions. When an expression has multiple operations that are of the same priority, we solve them from left to right.\\

Examples:
\begin{enumerate}
\item Simplify $(5\times 6)\times1^2 \div3-8+4$
\begin{mdframed}[style=TheoremFrame]
\textit{Solution:}
\begin{center}
\begin{tabular}{l r}
$(5\times 6)\times 1^2 \div 3-8+4$ &  Simplify the bracket\\
$ = 30 \times 1^2 \div 3-8+4$ &  Solve the exponent\\
$= 30 \times1 \div 3-8+4$ &  Multiply first two terms since they're on the left\\
$= 30 \div 3 -8+4$ &  Dividing because its the highest priority \\
$= 10 - 8 + 4$ & Subtracting since it comes first from the left\\
$= 2+4$ & \\
$= 6$ &\\
\end{tabular}
\end{center}

\end{mdframed}
\item Simplify $(6\times 2 - 5) \times \big((3+9)\times 4 \div 8 \big) \div 1^2-7^2$
\begin{mdframed}[style=TheoremFrame]
\textit{Solution:}
\begin{center}
\begin{tabular}{l r}
$(6\times 2 - 5) \times \big((3+9)\times 4 \div 8 \big) \div 1^2-7^2$ & Simplify the bracket within the bracket\\
$=(6\times 2 - 5) \times \big(12\times 4 \div 8 \big) \div 1^2-7^2$ & Multiply the first terms in the first bracket\\
$= (12 - 5) \times \big(12\times 4 \div 8 \big) \div 1^2-7^2$ & Finish simplifying the first bracket\\
$= 7 \times \big(12\times 4 \div 8 \big) \div 1^2-7^2$ & Multiply the first two terms in the bracket\\
$= 7 \times \big(48 \div 8 \big) \div 1^2-7^2$ & Finish the bracket\\
$= 7 \times 6 \div 1^2-7^2$ & Simplify both exponents\\
$= 7 \times 6 \div 1-49$ & Multiply first since it appears on the left\\
$= 42 \div 1-49$ & Divide since it has higher priority\\
$= 42-49$ & \\
$= -7$ & \\
\end{tabular}
\end{center}

\end{mdframed}
\item Simplify $\displaystyle{7^3 + 3\times (4 \times 5 - 2^2 -28 \div 7 +3) + 9 + \frac{3+5}{3-1}}$
\begin{mdframed}[style=TheoremFrame]
\textit{Solution:}
\begin{center}
\begin{tabular}{l r}
$\displaystyle{7^3 + 3\times (4 \times 5 - 2^2 -28 \div 7 +3) + 9 + \frac{3+5}{3-1}}$ & Rearrange the fraction \\
$= 7^3 + 3\times (4 \times 5 - 2^2 -28 \div 7 +3) + 9 + (5+3)\div(3-1)$ & Simplify the first bracket\\
$= 7^3 + 3\times (4 \times 5 - 4 -28 \div 7 +3) + 9 + (5+3)\div(3-1)$ &\\
$= 7^3 + 3\times (20 - 4 -28 \div 7 +3) + 9 + (5+3)\div(3-1)$ &\\
$= 7^3 + 3\times (20 - 4 -4 +3) + 9 + (5+3)\div(3-1)$ &\\
$= 7^3 + 3\times (16 -4 +3) + 9 + (5+3)\div(3-1)$ &\\
$= 7^3 + 3\times (12 +3) + 9 + (5+3)\div(3-1)$ &\\
$= 7^3 + 3\times 15 + 9 + (5+3)\div(3-1)$ & Final two brackets\\
$= 7^3 + 3\times 15 + 9 + 8\div(3-1)$ &\\
$= 7^3 + 3\times 15 + 9 + 8\div 2$ & Simplify exponent\\
$= 343 + 3\times 15 + 9 + 8\div 2$ & Multiplication\\
$= 343 + 45 + 9 + 8\div 2$ & Division\\
$= 343 + 45 + 9 + 4$ &\\
$= 388 + 9 + 4$ &\\
$= 397 + 4$ &\\
$= 401 $ & 
\end{tabular}
\end{center}

\end{mdframed}
\item Simplify $\displaystyle{(6\div (2+4)^{(2^2-4)})^2 + \big(6\times(2+1-2)\big)^2 \div 3}$
\begin{mdframed}[style=TheoremFrame]
\textit{Solution:}
\begin{center}
\begin{tabular}{l r}
$\displaystyle{(6\div (2+4)^{(2^2-4)})^2 + \big(6\times(2+1-2)\big)^2 \div 3}$ & Simplify the bracket in the exponent\\
$\displaystyle{(6\div (2+4)^{(4-4)})^2 + \big(6\times(2+1-2)\big)^2 \div 3}$ & Finish the subtraction in the exponent\\
$\displaystyle{(6\div (2+4)^{0})^2 + \big(6\times(2+1-2)\big)^2 \div 3}$ & Simplify bracket within first term\\
$\displaystyle{(6\div 6^{0})^2 + \big(6\times(2+1-2)\big)^2 \div 3}$ & Exponent within first bracket\\
$\displaystyle{(6\div 1)^2 + \big(6\times(2+1-2)\big)^2 \div 3}$ & Finish the first bracket\\
$\displaystyle{6^2 + \big(6\times(2+1-2)\big)^2 \div 3}$ & Simplify bracket within second term\\
$\displaystyle{6^2 + \big(6\times 1 \big)^2 \div 3}$ & Multiply terms within bracket\\
$\displaystyle{6^2 + 6^2 \div 3}$ & Calculate the exponents\\
$\displaystyle{36+ 36 \div 3}$ & Division has higher priority\\
$\displaystyle{36+ 12}$ & Finally add the remaining terms\\
$48$ & 
\end{tabular}
\end{center}
\end{mdframed}
\end{enumerate}
\newpage
Questions:
\begin{enumerate}
\item Simplify $2 \times (21+29) - 3^2 \times 7$
\vspace{6cm}
\item Simplify $7^2 - \big((3\times 6+3)\div 7\big)^3$
\vspace{6cm} 
\item Simplify $\displaystyle{6^{(3-2)} \times \big(3+25 \div (1+4) \big)}$
\end{enumerate}
\end{document}